rename handler_is → handler_spec, has_handler → handler_rpc_spec
Also move RPCSpec stuff into separate file, it is a layer on top of the basic rpc lib

src/program_proof/memkv/rpc_proof.v
@@ -92,7 +92,7 @@ Definition server_chan_inner (c: chan) γmap : iProp Σ :=
   "Hchan" ∷ c c↦ ms ∗
   "Hmessages" ∷ [∗ set] m ∈ ms, server_chan_inner_msg γmap m.
 
-Definition handler_is Γsrv (host:chan) (rpcid:u64) Spec : iProp Σ :=
+Definition handler_spec Γsrv (host:chan) (rpcid:u64) Spec : iProp Σ :=
   (∃ γ rpcdom,
    "#Hdom1" ∷ own (scset_name Γsrv) (to_agree (rpcdom)) ∗
    "%Hdom2" ∷ ⌜ rpcid ∈ rpcdom ⌝ ∗
@@ -101,100 +101,12 @@ Definition handler_is Γsrv (host:chan) (rpcid:u64) Spec : iProp Σ :=
   "#Hserver_inv" ∷ inv urpc_serverN (server_chan_inner host Γsrv)
 )%I.
 
-Global Instance handler_is_pers_instance γ host rpcid Spec :
-  Persistent (handler_is γ host rpcid Spec).
+Global Instance handler_spec_pers_instance γ host rpcid Spec :
+  Persistent (handler_spec γ host rpcid Spec).
 Proof. apply _. Qed.
 
 Definition handlers_dom Γsrv (d: gset u64) :=
   own (scset_name Γsrv) (to_agree (d : leibnizO (gset u64))).
-
-(* Higher-level interface for defining a handler with a given spec. *)
-Record RPCSpec :=
-  { spec_rpcid : u64;
-     spec_ty : Type;
-     spec_Pre : spec_ty → list u8 → iProp Σ;
-     spec_Post : spec_ty → list u8 → list u8 → iProp Σ }.
-
-Program Definition RPCSpec_Spec (spec : RPCSpec) : savedSpecO Σ (list u8) (list u8) :=
-  λ args, λne (Φ : list u8 -d> iPropO Σ), (∃ x : spec.(spec_ty),
-    spec.(spec_Pre) x args ∗ (∀ rep, spec.(spec_Post) x args rep -∗ Φ rep))%I.
-Next Obligation. (* FIXME solve_propert solved a very similar goal, why not this? *)
-  intros ??? Φ1 Φ2 HΦ. f_equiv.
-  intros x. f_equiv. f_equiv. intros rep. f_equiv. apply HΦ.
-Qed.
-
-Definition has_handler Γsrv (host:u64) (spec : RPCSpec) :=
-  handler_is Γsrv host spec.(spec_rpcid) (RPCSpec_Spec spec).
-
-(* We define a custom type for a list of RPC specs in order to state lemmas
-   about initializing a collection of handler_is facts. Unfortunately, using the
-   standard list type leads to a universe error if the spec_ty field contains an
-   iProp Σ, which turns out to be rather common. *)
-
-Inductive RPCSpecList : Type :=
-| spec_nil : RPCSpecList
-| spec_cons (x: RPCSpec) (l: RPCSpecList) : RPCSpecList.
-
-Fixpoint dom_RPCSpecList (l:  RPCSpecList) : gset u64 :=
-  match l with
-  | spec_nil => ∅
-  | spec_cons x l => {[ spec_rpcid x ]} ∪ dom_RPCSpecList l
-  end.
-
-Fixpoint handler_RPCSpecList γ host (l : RPCSpecList) :=
-  match l with
-  | spec_nil => True%I
-  | spec_cons x l =>
-    (has_handler γ host x ∗
-                handler_RPCSpecList γ host l)%I
-  end.
-
-Fixpoint RPCSpecList_wf (l : RPCSpecList) : Prop :=
-  match l with
-  | spec_nil => True
-  | spec_cons x l =>
-    (spec_rpcid x ∉ dom_RPCSpecList l) ∧ RPCSpecList_wf l
-  end.
-
-Lemma handler_is_init_list (host : chan) (specs: RPCSpecList) (Hwf: RPCSpecList_wf specs) :
-   host c↦ ∅ ={⊤}=∗ ∃ γ,
-   handlers_dom γ (dom_RPCSpecList specs) ∗
-   handler_RPCSpecList γ host specs.
-Proof.
-  iIntros "Hchan".
-  iMod (map_init (∅ : gmap u64 gname)) as (γmap) "Hmap_ctx".
-  iMod (own_alloc (to_agree (dom_RPCSpecList specs : leibnizO (gset u64)))) as (γdom) "#Hdom".
-  { econstructor. }
-  set (Γsrv := {| scmap_name := γmap; scset_name := γdom |}).
-  iMod (inv_alloc urpc_serverN _ ((server_chan_inner host Γsrv)) with "[Hchan]") as "#Hinv".
-  { iNext. iExists _. iFrame.
-    rewrite big_sepS_empty //. }
-  iExists Γsrv.
-  iAssert (∀ specs', ⌜ RPCSpecList_wf specs' ⌝ ∗ ⌜ dom_RPCSpecList specs' ⊆  dom_RPCSpecList specs ⌝ →
-           |==> ∃ gnames : gmap u64 gname, ⌜ dom (gset _) gnames = dom_RPCSpecList specs' ⌝ ∗
-           map_ctx (scmap_name Γsrv) 1 gnames ∗
-           handler_RPCSpecList Γsrv host specs')%I with "[Hmap_ctx]" as "H"; last first.
-  { iMod ("H" with "[]") as (?) "(_&_&$)"; eauto. }
-  iIntros (specs').
-  iInduction specs' as [| hd spec] "IH".
-  { iIntros (?). iModIntro. iExists ∅. iFrame.
-    rewrite ?dom_empty_L //. }
-  { iIntros ((Hwf'&Hdom')).
-    iMod ("IH" with "[$] []") as (gnames Hdom) "(Hmap_ctx&Hmap)".
-    { iPureIntro. split.
-      - destruct Hwf' as (_&?); eauto.
-      - etransitivity; last eassumption. set_solver. }
-    iMod (saved_spec_alloc (RPCSpec_Spec hd)) as (γsave) "#Hsaved".
-    iMod (map_alloc_ro (spec_rpcid hd) γsave
-            with "Hmap_ctx") as "(Hmap_ctx&#Hsaved_name)"; auto.
-    { apply not_elem_of_dom. destruct (Hwf') as (?&?). rewrite Hdom. eauto. }
-    iExists _; iFrame. iModIntro.
-    iSplit.
-    { iPureIntro. rewrite ?dom_insert_L Hdom. set_solver. }
-    iExists _, _. iFrame "#".
-    { iPureIntro. simpl in Hdom'. set_solver. }
-  }
-Qed.
 
 End rpc_global_defs.
 
@@ -328,7 +240,7 @@ Qed.
 
 Definition rpc_handler_mapping (γ : server_chan_gnames) (host : u64) (handlers : gmap u64 val) : iProp Σ :=
   ([∗ map] rpcid↦handler ∈ handlers, ∃ Spec,
-      handler_is γ host rpcid Spec ∗
+      handler_spec γ host rpcid Spec ∗
       is_rpcHandler' handler Spec)%I.
 
 Lemma non_empty_rpc_handler_mapping_inv γ host handlers :
@@ -346,8 +258,8 @@ Proof.
   rewrite /rpc_handler_mapping big_sepM_insert //.
   iDestruct "Hmapping" as "(H&Hmapping)".
   destruct (decide (dom (gset _) m = ∅)) as [Hemp|Hemp].
-  { iNamed "H". iDestruct "H" as "(Hhandler_is&His_rpcHandler)".
-    iNamed "Hhandler_is". iFrame "% #".
+  { iNamed "H". iDestruct "H" as "(Hhandler_spec&His_rpcHandler)".
+    iNamed "Hhandler_spec". iFrame "% #".
     rewrite big_sepM_insert //. iSplitL "His_rpcHandler".
     { iExists Spec, _.
       iFrame "# ∗". }
@@ -356,9 +268,9 @@ Proof.
   iDestruct ("IH" with "[//] [$]") as "HIH".
   iNamed "HIH". iFrame "% #".
   rewrite big_sepM_insert //. iFrame "#".
-  { iNamed "H". iDestruct "H" as "(Hhandler_is&His_rpcHandler)".
-    rewrite /handler_is.
-    iDestruct "Hhandler_is" as (g0 rpcdom) "H".
+  { iNamed "H". iDestruct "H" as "(Hhandler_spec&His_rpcHandler)".
+    rewrite /handler_spec.
+    iDestruct "Hhandler_spec" as (g0 rpcdom) "H".
     iDestruct "H" as "(#Hdom1&%Hdom2&#Hspec_name&#Hspec_saved&H)".
     iExists _, _.  iFrame "# ∗".
   }
@@ -534,7 +446,7 @@ Lemma wp_StartRPCServer γ (host : u64) (handlers : gmap u64 val) (s : loc) (n:u
       handlers_complete γ handlers ∗
       own_RPCServer s handlers ∗
       [∗ map] rpcid ↦ handler ∈ handlers,
-      (∃ Spec, handler_is γ host rpcid Spec ∗ is_rpcHandler' handler Spec)
+      (∃ Spec, handler_spec γ host rpcid Spec ∗ is_rpcHandler' handler Spec)
   }}}
     RPCServer__Serve #s #host #n
   {{{
@@ -804,7 +716,7 @@ Lemma wp_RPCClient__Call γsmap (cl_ptr:loc) (rpcid:u64) (host:u64) req rep_out_
   {{{
       is_slice req byteT 1 reqData ∗
       rep_out_ptr ↦[slice.T byteT] dummy_sl_val ∗
-      handler_is γsmap host rpcid Spec ∗
+      handler_spec γsmap host rpcid Spec ∗
       RPCClient_own cl_ptr host ∗
       □(▷ Spec reqData Post)
   }}}
