src/program_proof/memkv/rpc_spec.v
@@ -1,0 +1,102 @@
+(** Pre-postcondition-style specs for RPCs
+(translated to the predicate transformer style of the underlying lib *)
+From Perennial.algebra Require Import auth_map.
+From Perennial.base_logic Require Import lib.ghost_map lib.saved_spec.
+From Perennial.program_proof Require Import grove_prelude.
+From Perennial.program_proof.memkv Require Import rpc_proof.
+
+Section rpc_global_defs.
+
+Context `{!rpcregG Σ}.
+Context `{HPRE: !gooseGlobalGS Σ}.
+
+(* Higher-level interface for defining a handler with a given spec. *)
+Record RPCSpec :=
+  { spec_rpcid : u64;
+    spec_ty : Type;
+    spec_Pre : spec_ty → list u8 → iProp Σ;
+    spec_Post : spec_ty → list u8 → list u8 → iProp Σ }.
+
+Program Definition RPCSpec_Spec (spec : RPCSpec) : savedSpecO Σ (list u8) (list u8) :=
+  λ args, λne (Φ : list u8 -d> iPropO Σ), (∃ x : spec.(spec_ty),
+    spec.(spec_Pre) x args ∗ (∀ rep, spec.(spec_Post) x args rep -∗ Φ rep))%I.
+Next Obligation. (* FIXME solve_propert solved a very similar goal, why not this? *)
+  intros ??? Φ1 Φ2 HΦ. f_equiv.
+  intros x. f_equiv. f_equiv. intros rep. f_equiv. apply HΦ.
+Qed.
+
+Definition handler_rpc_spec Γsrv (host:u64) (spec : RPCSpec) :=
+  handler_spec Γsrv host spec.(spec_rpcid) (RPCSpec_Spec spec).
+
+(* We define a custom type for a list of RPC specs in order to state lemmas
+   about initializing a collection of handler_is facts. Unfortunately, using the
+   standard list type leads to a universe error if the spec_ty field contains an
+   iProp Σ, which turns out to be rather common. *)
+
+Inductive RPCSpecList : Type :=
+| spec_nil : RPCSpecList
+| spec_cons (x: RPCSpec) (l: RPCSpecList) : RPCSpecList.
+
+Fixpoint dom_RPCSpecList (l:  RPCSpecList) : gset u64 :=
+  match l with
+  | spec_nil => ∅
+  | spec_cons x l => {[ spec_rpcid x ]} ∪ dom_RPCSpecList l
+  end.
+
+Fixpoint handler_RPCSpecList γ host (l : RPCSpecList) :=
+  match l with
+  | spec_nil => True%I
+  | spec_cons x l =>
+    (handler_rpc_spec γ host x ∗
+                handler_RPCSpecList γ host l)%I
+  end.
+
+Fixpoint RPCSpecList_wf (l : RPCSpecList) : Prop :=
+  match l with
+  | spec_nil => True
+  | spec_cons x l =>
+    (spec_rpcid x ∉ dom_RPCSpecList l) ∧ RPCSpecList_wf l
+  end.
+
+Lemma handler_is_init_list (host : chan) (specs: RPCSpecList) (Hwf: RPCSpecList_wf specs) :
+   host c↦ ∅ ={⊤}=∗ ∃ γ,
+   handlers_dom γ (dom_RPCSpecList specs) ∗
+   handler_RPCSpecList γ host specs.
+Proof.
+  iIntros "Hchan".
+  iMod (map_init (∅ : gmap u64 gname)) as (γmap) "Hmap_ctx".
+  iMod (own_alloc (to_agree (dom_RPCSpecList specs : leibnizO (gset u64)))) as (γdom) "#Hdom".
+  { econstructor. }
+  set (Γsrv := {| scmap_name := γmap; scset_name := γdom |}).
+  iMod (inv_alloc urpc_serverN _ ((server_chan_inner host Γsrv)) with "[Hchan]") as "#Hinv".
+  { iNext. iExists _. iFrame.
+    rewrite big_sepS_empty //. }
+  iExists Γsrv.
+  iAssert (∀ specs', ⌜ RPCSpecList_wf specs' ⌝ ∗ ⌜ dom_RPCSpecList specs' ⊆  dom_RPCSpecList specs ⌝ →
+           |==> ∃ gnames : gmap u64 gname, ⌜ dom (gset _) gnames = dom_RPCSpecList specs' ⌝ ∗
+           map_ctx (scmap_name Γsrv) 1 gnames ∗
+           handler_RPCSpecList Γsrv host specs')%I with "[Hmap_ctx]" as "H"; last first.
+  { iMod ("H" with "[]") as (?) "(_&_&$)"; eauto. }
+  iIntros (specs').
+  iInduction specs' as [| hd spec] "IH".
+  { iIntros (?). iModIntro. iExists ∅. iFrame.
+    rewrite ?dom_empty_L //. }
+  { iIntros ((Hwf'&Hdom')).
+    iMod ("IH" with "[$] []") as (gnames Hdom) "(Hmap_ctx&Hmap)".
+    { iPureIntro. split.
+      - destruct Hwf' as (_&?); eauto.
+      - etransitivity; last eassumption. set_solver. }
+    iMod (saved_spec_alloc (RPCSpec_Spec hd)) as (γsave) "#Hsaved".
+    iMod (map_alloc_ro (spec_rpcid hd) γsave
+            with "Hmap_ctx") as "(Hmap_ctx&#Hsaved_name)"; auto.
+    { apply not_elem_of_dom. destruct (Hwf') as (?&?). rewrite Hdom. eauto. }
+    iExists _; iFrame. iModIntro.
+    iSplit.
+    { iPureIntro. rewrite ?dom_insert_L Hdom. set_solver. }
+    iExists _, _. iFrame "#".
+    { iPureIntro. simpl in Hdom'. set_solver. }
+  }
+Qed.
+
+
+End rpc_global_defs.
